Start adding standalone versions of specs.

examples/nsl_dh/impl.v
@@ -73,7 +73,7 @@ Definition responder_recv_msg1 : val := λ: "c" "skR",
   guard: is_aenc_key "pkI" in
   SOME ("ga", "pkI").
 
-Definition responder_send_msg2 : val := λ: "c" "skR" "ga" "pkI" "N",
+Definition responder_send_msg2 : val := λ: "c" "skR" "pkI" "N" "ga",
   let: "pkR" := pkey "skR" in
   let: "keys" := mk_dh_keys #() in
   let: "b"    := Fst "keys" in
@@ -83,10 +83,24 @@ Definition responder_send_msg2 : val := λ: "c" "skR" "ga" "pkI" "N",
   send "c" "m2";;
   "keys".
 
-Definition responder_recv_msg3 : val := λ: "c" "skR" "pkI" "b" "gb" "ga",
+Definition responder_recv_msg3 : val := λ: "c" "skR" "pkI" "ga" "b" "gb",
   let: "pkR" := pkey "skR" in
   bind: "m3" := adec "skR" (Tag $ nsl_dhN.@"m3") (recv "c") in
   guard: eq_term "gb" "gb'" in
   let: "gab"    := texp "ga" "b" in
   let: "secret" := term_of_list ["pkI"; "pkR"; "ga"; "gb"; "gab"] in
   SOME (derive_senc_key "secret").
+
+Definition responder_listen := responder_recv_msg1.
+
+Definition responder_confirm : val := λ: "c" "skR" "pkI" "N" "ga",
+  let: "keys" := responder_send_msg2 "c" "skR" "pkI" "N" "ga" in
+  let: "b" := Fst "keys" in
+  let: "gb" := Snd "keys" in
+  responder_recv_msg3 "c" "skR" "pkI" "N" "ga" "b" "gb".
+
+Definition responder : val := λ: "c" "skR" "N",
+  bind: "info" := responder_listen "c" "skR" in
+  let: "ga" := Fst "info" in
+  let: "pkI" := Snd "info" in
+  responder_confirm "c" "skR" "pkI" "N" "ga".
